WIP

demo/owned_heap/OHAllocTarget.c
@@ -15,5 +15,30 @@ void set(int *key, int val) {
   *key = val;
 }
 
-//TODO: void init(int* ptr);
-//map(void *f) { apply f } .. ?
+
+
+
+
+void delete(int *key) {
+  free(key);
+}
+
+typedef int (*int_func_int) (int);
+
+void map(int *key, int_func_int f) {
+  *key = f(*key);
+}
+
+void publicize(int *key) {
+}
+
+void privatize(int *key) {
+}
+
+void init(int *key) {
+  *key = 0;
+}
+
+void fini(int *key) {
+}
+
