demo/owned_heap/SimMemSV.v
@@ -17,6 +17,205 @@ Set Implicit Arguments.
 
 
 
+Lemma iff_eta
+      (P Q: Prop)
+      (EQ: P = Q)
+  :
+    <<EQ: P <-> Q>>
+.
+Proof. clarify. Qed.
+
+Lemma and_eta
+      (P0 P1 Q0 Q1: Prop)
+      (EQ0: P0 = P1)
+      (EQ1: Q0 = Q1)
+  :
+    <<EQ: (P0 /\ Q0) = (P1 /\ Q1)>>
+.
+Proof. clarify. Qed.
+
+Ltac smart_intro T :=
+  intro;
+  let x := match goal with
+           | [ H: _ |- _ ] => H
+           end
+  in
+  (* idtac x; *)
+  on_last_hyp ltac:(fun id => revert id);
+
+  let name := fresh "H" in
+  intro name;
+  let y := match goal with
+           | [ H: _ |- _ ] => H
+           end
+  in
+  (* idtac y; *)
+  on_last_hyp ltac:(fun id => revert id);
+
+  tryif (check_equal x y)
+  then
+    let name := fresh T in intro name
+    (* (tryif check_hyp T *)
+    (*   then (tryif check_hyp "U" *)
+    (*          then (tryif (check_hyp "V") *)
+    (*                 then (let name := (fresh "W") in intro name) *)
+    (*                 else (let name := (fresh "V") in intro name)) *)
+    (*          else (let name := (fresh "U") in intro name)) *)
+    (*   else (let name := (fresh "T") in intro name)) *)
+
+    (* (tryif check_hyp string:("T") *)
+    (*   then (tryif check_hyp string:("U") *)
+    (*          then (tryif (check_hyp string:("V")) *)
+    (*                 then (intro W) *)
+    (*                 else (intro V)) *)
+    (*          else (intro U)) *)
+    (*   else (intro T)) *)
+
+    (* let T := fresh "T" in *)
+    (* let U := fresh "U" in *)
+    (* let V := fresh "V" in *)
+    (* let W := fresh "W" in *)
+    (* (tryif check_hyp T *)
+    (*   then (tryif check_hyp U *)
+    (*          then (tryif (check_hyp V) *)
+    (*                 then (intro W) *)
+    (*                 else (intro V)) *)
+    (*          else (intro U)) *)
+    (*   else (intro T)) *)
+  else intro x
+
+  (* match x with *)
+  (* | y => let name := fresh T in *)
+  (*        intro name *)
+  (* | _ => intro x *)
+  (* end *)
+.
+
+Tactic Notation "ii" "as" ident(a) := repeat (let name := fresh a in intro name).
+(* Ltac sii := repeat (smart_intro "X"). *)
+Tactic Notation "sii" ident(X) := repeat (smart_intro X).
+Goal forall (t: True), True -> forall (u: True), True -> False.
+Proof.
+  sii T.
+  clear t. clear T. clear u. clear T0.
+Abort.
+Hint Unfold privmod_others.
+
+
+
+
+
+Section FROZEN.
+
+Inductive frozen (f_old f_new: meminj) (bound_src bound_tgt: block): Prop :=
+| frozen_intro
+    (NEW_IMPLIES_OUTSIDE:
+       forall b_src b_tgt delta
+              (NEW: f_old b_src = None /\ f_new b_src = Some(b_tgt, delta)),
+         <<OUTSIDE_SRC: (bound_src <= b_src)%positive>> /\ <<OUTSIDE_TGT: (bound_tgt <= b_tgt)%positive>>).
+
+Remark inject_separated_frozen: forall f_old f_new m_src m_tgt,
+    Events.inject_separated f_old f_new m_src m_tgt <->
+    frozen f_old f_new m_src.(Mem.nextblock) m_tgt.(Mem.nextblock).
+Proof.
+  unfold Events.inject_separated, Mem.valid_block in *. split; i.
+  - econs; eauto. i. des. hexploit H; eauto. i; des. splits; xomega.
+  - inv H. exploit NEW_IMPLIES_OUTSIDE; eauto. i; des. split; xomega.
+Qed.
+
+Lemma frozen_preserves_src
+      f_old f_new bound_src bound_tgt b_src
+      (INJECT: inject_incr f_old f_new)
+      (FROZEN: frozen f_old f_new bound_src bound_tgt)
+      (INSIDE: (b_src < bound_src)%positive):
+    <<PRESERVED: f_old b_src = f_new b_src>>.
+Proof.
+  inv FROZEN. destruct (f_old b_src) eqn:T0; ss; destruct (f_new b_src) eqn:T1; ss.
+  - destruct p, p0; ss. exploit INJECT; eauto; []; i; des. clarify.
+  - destruct p; ss. exploit INJECT; eauto; []; i; des. clarify.
+  - destruct p; ss. exploit NEW_IMPLIES_OUTSIDE; eauto; []; i; des. exfalso. xomega.
+Qed.
+
+Lemma frozen_preserves_tgt
+      f_old f_new bound_src bound_tgt b_tgt
+      (INJECT: inject_incr f_old f_new)
+      (FROZEN: frozen f_old f_new bound_src bound_tgt)
+      (INSIDE: (b_tgt < bound_tgt)%positive):
+    <<PRESERVED: forall b_src delta (NOW: f_new b_src = Some (b_tgt, delta)),
+      <<OLD: f_old b_src = Some (b_tgt, delta)>> >>.
+Proof.
+  inv FROZEN. ii. destruct (f_old b_src) eqn:T; ss.
+  - destruct p; ss. exploit INJECT; eauto; []; i; des. clarify.
+  - exfalso. exploit NEW_IMPLIES_OUTSIDE; eauto; []; i; des. xomega.
+Qed.
+
+Lemma frozen_shortened
+      f_old f_new bd_src0 bd_tgt0 bd_src1 bd_tgt1
+      (FROZEN: frozen f_old f_new bd_src0 bd_tgt0)
+      (SHORT_SRC: (bd_src1 <= bd_src0)%positive)
+      (SHORT_TGT: (bd_tgt1 <= bd_tgt0)%positive):
+    <<FROZEN: frozen f_old f_new bd_src1 bd_tgt1>>.
+Proof.
+  inv FROZEN. econs; eauto. ii. des.
+  hexploit NEW_IMPLIES_OUTSIDE; eauto; []; i; des. clear NEW_IMPLIES_OUTSIDE.
+  split; ss; red; etransitivity; eauto.
+Qed.
+
+Lemma frozen_refl: forall f bound_src bound_tgt,
+    <<FROZEN: frozen f f bound_src bound_tgt>>.
+Proof. econs; eauto. i; des. clarify. Qed.
+
+Lemma loc_unmapped_frozen
+      F F' fbound_src fbound_tgt b ofs
+      (FROZEN : frozen F F' fbound_src fbound_tgt)
+      (BOUND: Plt b fbound_src)
+      (UNMAPPED: loc_unmapped F b ofs):
+    loc_unmapped F' b ofs.
+Proof.
+  unfold loc_unmapped in *.
+  destruct (F' b) eqn:T; ss. destruct p; ss.
+  inv FROZEN. exploit NEW_IMPLIES_OUTSIDE; eauto. i; des. xomega.
+Qed.
+
+Lemma loc_out_of_reach_frozen
+      F F' fbound_src fbound_tgt b ofs m0 m1
+      (INCR: inject_incr F F')
+      (FROZEN : frozen F F' fbound_src fbound_tgt)
+      (BOUND: Plt b fbound_tgt)
+      (UNMAPPED: loc_out_of_reach F m0 b ofs)
+      (MAXPERM: forall b0 delta (MAPPED: F b0 = Some (b, delta)),
+          Mem.perm m1 b0 (ofs - delta) Max Nonempty -> Mem.perm m0 b0 (ofs - delta) Max Nonempty):
+    loc_out_of_reach F' m1 b ofs.
+Proof.
+  unfold loc_out_of_reach in *. i. exploit frozen_preserves_tgt; eauto. i. des. hexploit UNMAPPED; eauto.
+Qed.
+
+End FROZEN.
+
+Inductive frozen_incr (bound_src bound_tgt: block) (f_old f_new: meminj): Prop :=
+| frozen_incr_intro
+    (FROZEN: frozen f_old f_new bound_src bound_tgt)
+    (INCR: inject_incr f_old f_new)
+.
+
+Global Program Instance frozen_incr_PreOrder (bound_src bound_tgt: block):
+  PreOrder (frozen_incr bound_src bound_tgt).
+Next Obligation.
+  econs; eauto. econs; eauto. i; des. clarify.
+Qed.
+Next Obligation.
+  ii. inv H. inv H0. econs; eauto; cycle 1.
+  { eapply inject_incr_trans; et. }
+  econs; eauto. inv FROZEN. inv FROZEN0. i; des.
+  destruct (y b_src) eqn:T.
+  - destruct p; ss. exploit NEW_IMPLIES_OUTSIDE; et. i; des. esplits; et; try xomega.
+    exploit INCR0; et. i; des. clarify.
+  - exploit NEW_IMPLIES_OUTSIDE0; et.
+Qed.
+
+
+
+
 
 Inductive ownership: Type :=
 | privmod (mi: string)
@@ -56,11 +255,10 @@ Definition ownership_mem_bool (ptt: partition) (ons: ownership): block -> Z -> b
   fun b ofs => ownership_dec (ptt b ofs) ons
 .
 
-Definition ownership_mem (ptt: partition) (ons: ownership): block -> Z -> Prop :=
+Definition ons_mem (ptt: partition) (ons: ownership): block -> Z -> Prop :=
   fun b ofs => (ptt b ofs) = ons
 .
-
-Hint Unfold ownership_mem.
+Hint Unfold ons_mem.
 
 
 Section MEMINJ.
@@ -72,20 +270,14 @@ Record t' := mk {
   src: mem;
   tgt: mem;
   inj: meminj;
+  ge_nb_src: block;
+  ge_nb_tgt: block;
   ptt_src: partition;
   ptt_tgt: partition;
 }.
 
 Definition valid_blocks (m: mem): block -> Z -> Prop := fun b _ => (Mem.valid_block m) b.
 Hint Unfold valid_blocks.
-
-Definition external_src (sm: t'): block -> Z -> Prop :=
-  fun b ofs => sm.(ptt_src) b ofs = external
-.
-
-Definition external_tgt (sm: t'): block -> Z -> Prop :=
-  fun b ofs => sm.(ptt_tgt) b ofs = external
-.
 
 Definition private_src (sm: t'): block -> Z -> Prop :=
   loc_unmapped sm.(inj) /2\ (valid_blocks sm.(src)).
@@ -105,31 +297,38 @@ Qed.
 Inductive wf' (sm0: t'): Prop :=
 | wf_intro
     (PUBLIC: Mem.inject sm0.(inj) sm0.(src) sm0.(tgt))
+    (GENBSRC: (sm0.(ge_nb_src) <= sm0.(src).(Mem.nextblock))%positive)
+    (GENBTGT: (sm0.(ge_nb_tgt) <= sm0.(tgt).(Mem.nextblock))%positive)
     (* (PTTSRC: (public_src sm0) = (ownership_mem sm0.(ptt_src) pub)) *)
     (* (PTTTGT: (public_tgt sm0) = (ownership_mem sm0.(ptt_tgt) pub)) *)
-    (PTTSRC: all2 ((public_src sm0) <2> (ownership_mem sm0.(ptt_src) pub)))
-    (PTTTGT: all2 ((public_tgt sm0) <2> (ownership_mem sm0.(ptt_tgt) pub)))
+    (* (PTTSRC: all2 ((public_src sm0) <2> (ownership_mem sm0.(ptt_src) pub))) *)
+    (* (PTTTGT: all2 ((public_tgt sm0) <2> (ownership_mem sm0.(ptt_tgt) pub))) *)
+    (PTTSRC: (public_src sm0) <2= (ons_mem sm0.(ptt_src) pub))
+    (PTTTGT: (public_tgt sm0) <2= (ons_mem sm0.(ptt_tgt) pub))
 .
 
-Inductive le' (mrel0 mrel1: t'): Prop :=
+Inductive le' (sm0 sm1: t'): Prop :=
 | le_intro
-    (INCR: inject_incr mrel0.(inj) mrel1.(inj))
-    (UNCHSRC: Mem.unchanged_on (external_src mrel0) mrel0.(src) mrel1.(src))
-    (UNCHTGT: Mem.unchanged_on (external_tgt mrel0) mrel0.(tgt) mrel1.(tgt))
-    (PUBSRC: (public_src mrel0) <2= (public_src mrel1))
-    (PUBTGT: (public_tgt mrel0) <2= (public_tgt mrel1))
-    (EXTSRC: (external_src mrel0) <2= (external_src mrel1))
-    (EXTTGT: (external_tgt mrel0) <2= (external_tgt mrel1))
-    (PMSRC: forall mi, (ownership_mem mrel0.(ptt_src) (privmod mi)) <2=
-                       (ownership_mem mrel1.(ptt_src) (privmod mi)))
-    (PMTGT: forall mi, (ownership_mem mrel0.(ptt_tgt) (privmod mi)) <2=
-                       (ownership_mem mrel1.(ptt_tgt) (privmod mi)))
+    (GENBSRC: sm0.(ge_nb_src) = sm1.(ge_nb_src))
+    (GENBTGT: sm0.(ge_nb_tgt) = sm1.(ge_nb_tgt))
+    (FINCR: frozen_incr (sm0.(ge_nb_src)) (sm0.(ge_nb_tgt)) sm0.(inj) sm1.(inj))
+    (* (INCR: inject_incr sm0.(inj) sm1.(inj)) *)
+    (UNCHSRC: Mem.unchanged_on (ons_mem sm0.(ptt_src) external) sm0.(src) sm1.(src))
+    (UNCHTGT: Mem.unchanged_on (ons_mem sm0.(ptt_tgt) external) sm0.(tgt) sm1.(tgt))
+    (PUBSRC: (ons_mem sm0.(ptt_src) pub) <2= (ons_mem sm1.(ptt_src) pub))
+    (PUBTGT: (ons_mem sm0.(ptt_tgt) pub) <2= (ons_mem sm1.(ptt_tgt) pub))
+    (EXTSRC: (ons_mem sm0.(ptt_src) external) <2= (ons_mem sm1.(ptt_src) external))
+    (EXTTGT: (ons_mem sm0.(ptt_tgt) external) <2= (ons_mem sm1.(ptt_tgt) external))
+    (PMSRC: forall mi, (ons_mem sm0.(ptt_src) (privmod mi)) <2= (ons_mem sm1.(ptt_src) (privmod mi)))
+    (PMTGT: forall mi, (ons_mem sm0.(ptt_tgt) (privmod mi)) <2= (ons_mem sm1.(ptt_tgt) (privmod mi)))
     (MAXSRC: forall b ofs
-        (VALID: Mem.valid_block mrel0.(src) b),
-        <<MAX: Mem.perm mrel1.(src) b ofs Max <1= Mem.perm mrel0.(src) b ofs Max>>)
+        (VALID: Mem.valid_block sm0.(src) b),
+        <<MAX: Mem.perm sm1.(src) b ofs Max <1= Mem.perm sm0.(src) b ofs Max>>)
     (MAXTGT: forall b ofs
-        (VALID: Mem.valid_block mrel0.(tgt) b),
-        <<MAX: Mem.perm mrel1.(tgt) b ofs Max <1= Mem.perm mrel0.(tgt) b ofs Max>>)
+        (VALID: Mem.valid_block sm0.(tgt) b),
+        <<MAX: Mem.perm sm1.(tgt) b ofs Max <1= Mem.perm sm0.(tgt) b ofs Max>>)
+    (** tried to minimize it (don't require FROZEN),
+but because of volatile condiiton in symbols_inject, I think we need it **)
 .
 
 Global Program Instance le'_PreOrder: RelationClasses.PreOrder le'.
@@ -139,7 +338,7 @@ Qed.
 Next Obligation.
   ii. inv H; inv H0. des; clarify.
   econs; eauto with mem congruence.
-  + eapply inject_incr_trans; eauto.
+  + etrans; et. eauto with congruence.
   + eapply Mem.unchanged_on_trans.
     { eauto with congruence. }
     eapply Mem.unchanged_on_implies; eauto.
@@ -167,7 +366,8 @@ Definition lift_ptt (ptt: partition): partition :=
 .
 
 Definition lift' (mrel0: t'): t' :=
-  (mk mrel0.(src) mrel0.(tgt) mrel0.(inj)
+  (mk (mrel0.(src)) (mrel0.(tgt)) (mrel0.(inj))
+      (mrel0.(ge_nb_src)) (mrel0.(ge_nb_tgt))
       (lift_ptt (ptt_src mrel0)) (lift_ptt (ptt_tgt mrel0))
   ).
 
@@ -187,6 +387,7 @@ Definition unlift_ptt (ptt0 ptt1: partition): partition :=
 
 Definition unlift' (mrel0 mrel1: t'): t' :=
   (mk mrel1.(src) mrel1.(tgt) mrel1.(inj)
+      (mrel0.(ge_nb_src)) (mrel0.(ge_nb_tgt))
       (unlift_ptt (ptt_src mrel0) (ptt_src mrel1)) (unlift_ptt (ptt_tgt mrel0) (ptt_tgt mrel1))
   ).
 
@@ -196,16 +397,20 @@ Lemma unlift_spec : forall mrel0 mrel1 : t',
                   le' (lift' mrel0) mrel1 -> wf' mrel0 -> le' mrel0 (unlift' mrel0 mrel1).
 Proof.
   i. inv H; ss. econs; ss; eauto; ii; des; ss.
-  - eapply Mem.unchanged_on_implies; eauto. ii. unfold external_src in *. ss. unfold lift_ptt. des_ifs.
-  - eapply Mem.unchanged_on_implies; eauto. ii. unfold external_tgt in *. ss. unfold lift_ptt. des_ifs.
-  - clear - EXTSRC PR. unfold external_src in *. ss. unfold lift_ptt, unlift_ptt in *.
+  - eapply Mem.unchanged_on_implies; eauto. ii. unfold ons_mem in *. ss. unfold lift_ptt. des_ifs.
+  - eapply Mem.unchanged_on_implies; eauto. ii. unfold ons_mem in *. ss. unfold lift_ptt. des_ifs.
+  - clear - PUBSRC PR. unfold ons_mem in *. ss. unfold lift_ptt, unlift_ptt in *.
+    specialize (PUBSRC x0 x1). ss. rewrite PR in *. rewrite PUBSRC; ss.
+  - clear - PUBTGT PR. unfold ons_mem in *. ss. unfold lift_ptt, unlift_ptt in *.
+    specialize (PUBTGT x0 x1). ss. rewrite PR in *. rewrite PUBTGT; ss.
+  - clear - EXTSRC PR. unfold ons_mem in *. ss. unfold lift_ptt, unlift_ptt in *.
     specialize (EXTSRC x0 x1). ss. rewrite PR in *. rewrite EXTSRC; ss.
-  - clear - EXTTGT PR. unfold external_tgt in *. ss. unfold lift_ptt, unlift_ptt in *.
+  - clear - EXTTGT PR. unfold ons_mem in *. ss. unfold lift_ptt, unlift_ptt in *.
     specialize (EXTTGT x0 x1). ss. rewrite PR in *. rewrite EXTTGT; ss.
-  - clear - PMSRC PR. unfold ownership_mem in *. des_sumbool. ss. unfold lift_ptt, unlift_ptt in *.
+  - clear - PMSRC PR. unfold ons_mem in *. des_sumbool. ss. unfold lift_ptt, unlift_ptt in *.
     specialize (PMSRC mi x0 x1). ss. rewrite PR in *.
     hexploit1 PMSRC. { des_sumbool; ss. } des_sumbool. des_ifs.
-  - clear - PMTGT PR. unfold ownership_mem in *. des_sumbool. ss. unfold lift_ptt, unlift_ptt in *.
+  - clear - PMTGT PR. unfold ons_mem in *. des_sumbool. ss. unfold lift_ptt, unlift_ptt in *.
     specialize (PMTGT mi x0 x1). ss. rewrite PR in *.
     hexploit1 PMTGT. { des_sumbool; ss. } des_sumbool. des_ifs.
 Qed.
@@ -216,52 +421,34 @@ Lemma unlift_wf : forall mrel0 mrel1 : t',
 Proof.
   i. inv H. inv H0. inv H1. des; clarify.
   econs; ss.
+  - etrans; et. eapply Mem.unchanged_on_nextblock; et.
+  - etrans; et. eapply Mem.unchanged_on_nextblock; et.
   -
     intros b ofs.
-    unfold public_src, private_src. ss. split; i.
+    unfold public_src, private_src. unfold ons_mem in *. ss. i.
     + unfold unlift_ptt.
       specialize (PTTSRC0 b ofs).
-      apply proj1 in PTTSRC0.
-      apply not_and_or in H. des.
-      * unfold loc_unmapped in *. unfold ownership_mem. des_sumbool.
+      apply not_and_or in PR. des.
+      * unfold loc_unmapped in *.
         exploit PTTSRC0.
-        { unfold public_src. ii. eapply H. unfold private_src in *. des; ss. }
-        intro T. unfold ownership_mem in *. des_sumbool. rewrite T. ss.
+        { unfold public_src. ii. eapply PR. unfold private_src in *. des; ss. }
+        intro T. rewrite T. ss.
       * exploit PTTSRC0.
-        { unfold public_src. ii. eapply H. unfold private_src in *. des; ss. }
-        intro T. unfold ownership_mem in *. des_sumbool. rewrite T. ss.
-    + unfold unlift_ptt in *.
-      specialize (PTTSRC0 b ofs).
-      apply proj2 in PTTSRC0.
-      eapply or_not_and.
-      unfold loc_unmapped in *. unfold ownership_mem in *. des_sumbool.
-      des_ifs.
-      hexploit PTTSRC0.
-      { des_sumbool. ss. }
-      intro T. unfold public_src, private_src in T. apply not_and_or in T. ss.
+        { unfold public_src. ii. eapply PR. unfold private_src in *. des; ss. }
+        intro T. rewrite T. ss.
   -
     intros b ofs.
-    unfold public_tgt, private_tgt. ss. split; i.
+    unfold public_tgt, private_tgt. unfold ons_mem in *. ss. i.
     + unfold unlift_ptt.
       specialize (PTTTGT0 b ofs).
-      apply proj1 in PTTTGT0.
-      apply not_and_or in H. des.
-      * unfold loc_unmapped in *. unfold ownership_mem. des_sumbool.
+      apply not_and_or in PR. des.
+      * unfold loc_unmapped in *.
         exploit PTTTGT0.
-        { unfold public_tgt. ii. eapply H. unfold private_tgt in *. des; ss. }
-        intro T. unfold ownership_mem in *. des_sumbool. rewrite T. ss.
+        { unfold public_tgt. ii. eapply PR. unfold private_tgt in *. des; ss. }
+        intro T. rewrite T. ss.
       * exploit PTTTGT0.
-        { unfold public_tgt. ii. eapply H. unfold private_tgt in *. des; ss. }
-        intro T. unfold ownership_mem in *. des_sumbool. rewrite T. ss.
-    + unfold unlift_ptt in *.
-      specialize (PTTTGT0 b ofs).
-      apply proj2 in PTTTGT0.
-      eapply or_not_and.
-      unfold loc_unmapped in *. unfold ownership_mem in *. des_sumbool.
-      des_ifs.
-      hexploit PTTTGT0.
-      { des_sumbool. ss. }
-      intro T. unfold public_tgt, private_tgt in T. apply not_and_or in T. ss.
+        { unfold public_tgt. ii. eapply PR. unfold private_tgt in *. des; ss. }
+        intro T. rewrite T. ss.
 Qed.
 
 (* Lemma after_private_src *)
@@ -302,7 +489,7 @@ Hint Unfold public_src public_tgt.
 Section MEMINJ.
 
 Definition update (sm0: t') (src tgt: mem) (inj: meminj): t' :=
-  mk src tgt inj (sm0.(ptt_src)) (sm0.(ptt_tgt))
+  mk src tgt inj sm0.(ge_nb_src) sm0.(ge_nb_tgt) (sm0.(ptt_src)) (sm0.(ptt_tgt))
 .
 Hint Unfold update.
 (* Notation "sm0 '.(update_tgt)' tgt" := (sm0.(update) sm0.(src) tgt sm0.(inj)) (at level 50). *)
@@ -314,22 +501,25 @@ Hint Unfold private_src private_tgt valid_blocks.
 
 Inductive lepriv (sm0 sm1: t'): Prop :=
 | lepriv_intro
-    (INCR: inject_incr sm0.(inj) sm1.(inj))
-    (PUBSRC: (public_src sm0) <2= (public_src sm1))
-    (PUBTGT: (public_tgt sm0) <2= (public_tgt sm1))
-    (PMSRC: forall mi, (ownership_mem sm0.(ptt_src) (privmod mi)) <2=
-                       (ownership_mem sm1.(ptt_src) (privmod mi)))
-    (PMTGT: forall mi, (ownership_mem sm0.(ptt_tgt) (privmod mi)) <2=
-                       (ownership_mem sm1.(ptt_tgt) (privmod mi)))
+    (FINCR: frozen_incr (sm0.(ge_nb_src)) (sm0.(ge_nb_tgt)) sm0.(inj) sm1.(inj))
+    (GENBSRC: sm0.(ge_nb_src) = sm1.(ge_nb_src))
+    (GENBTGT: sm0.(ge_nb_tgt) = sm1.(ge_nb_tgt))
+    (* (PUBSRC: (public_src sm0) <2= (public_src sm1)) *)
+    (* (PUBTGT: (public_tgt sm0) <2= (public_tgt sm1)) *)
+    (PUBSRC: (ons_mem sm0.(ptt_src) pub) <2= (ons_mem sm1.(ptt_src) pub))
+    (PUBTGT: (ons_mem sm0.(ptt_tgt) pub) <2= (ons_mem sm1.(ptt_tgt) pub))
+    (PMSRC: forall mi, (ons_mem sm0.(ptt_src) (privmod mi)) <2= (ons_mem sm1.(ptt_src) (privmod mi)))
+    (PMTGT: forall mi, (ons_mem sm0.(ptt_tgt) (privmod mi)) <2= (ons_mem sm1.(ptt_tgt) (privmod mi)))
 .
 
 Global Program Instance lepriv_PreOrder: RelationClasses.PreOrder lepriv.
 Next Obligation.
   ii. econs; eauto.
+  refl.
 Qed.
 Next Obligation.
   ii. inv H; inv H0. des; clarify. econs; eauto with mem congruence.
-  + eapply inject_incr_trans; eauto.
+  + etrans; et. rp; et.
   + etrans; et.
   + etrans; et.
 Qed.
@@ -362,7 +552,7 @@ Next Obligation. rename H into LE. inv LE. econs; et. Qed.
 (* Next Obligation. *)
 (*   eapply unlift_wf; eauto. *)
 (* Qed. *)
-Next Obligation. ii. inv MLE. eapply val_inject_incr; eauto. Qed.
+Next Obligation. ii. inv MLE. eapply val_inject_incr; try apply FINCR; eauto. Qed.
 Next Obligation.
   do 2 (apply Axioms.functional_extensionality; i). apply prop_ext1. split; i; ss; clarify.
   - ginduction x; ii; inv H; ss. econs; eauto.
@@ -376,33 +566,14 @@ Next Obligation. ii. eapply Mem.unchanged_on_implies; et. Qed.
 
 
 
-Lemma iff_eta
-      (P Q: Prop)
-      (EQ: P = Q)
-  :
-    <<EQ: P <-> Q>>
-.
-Proof. clarify. Qed.
-
-Lemma and_eta
-      (P0 P1 Q0 Q1: Prop)
-      (EQ0: P0 = P1)
-      (EQ1: Q0 = Q1)
-  :
-    <<EQ: (P0 /\ Q0) = (P1 /\ Q1)>>
-.
-Proof. clarify. Qed.
-
 Global Program Instance SimMemSVLift : SimMemLift.class SimMemSV :=
 { lift := lift';
   unlift := unlift';
 }.
 Next Obligation.
   inv H. econs; et.
-  - unfold lift', lift_ptt. ss. unfold public_src, private_src in *. ss. ii. etrans; et.
-    unfold ownership_mem. split; i; des_ifs.
-  - unfold lift', lift_ptt. ss. unfold public_tgt, private_tgt in *. ss. ii. etrans; et.
-    unfold ownership_mem. split; i; des_ifs.
+  - etrans; et. unfold lift', ons_mem. ss. unfold lift_ptt; ss. ii. des_ifs.
+  - etrans; et. unfold lift', ons_mem. ss. unfold lift_ptt; ss. ii. des_ifs.
 Qed.
 Next Obligation.
   eapply func_ext2. intros b ofs. unfold lift_ptt. des_ifs.
@@ -420,13 +591,19 @@ Next Obligation. eapply unlift_spec; et. Qed.
 Next Obligation. eapply unlift_wf; eauto. Qed.
 Next Obligation.
   inv MWF. destruct sm0; ss. econs; ss; et.
-  - ii. unfold ownership_mem in *. unfold lift_ptt. des_ifs.
-  - ii. unfold ownership_mem in *. unfold lift_ptt. des_ifs.
+  - refl.
+  - ii. unfold ons_mem in *. unfold lift_ptt. des_ifs.
+  - ii. unfold ons_mem in *. unfold lift_ptt. des_ifs.
+  - ii. unfold ons_mem in *. unfold lift_ptt. des_ifs.
+  - ii. unfold ons_mem in *. unfold lift_ptt. des_ifs.
 Qed.
 Next Obligation.
   inv MWF. inv MLE. inv MLIFT. econs; ss; et; try congruence.
-  - ii. unfold ownership_mem in *. unfold unlift_ptt. des_ifs.
-  - ii. unfold ownership_mem in *. unfold unlift_ptt. des_ifs.
+  - refl.
+  - ii. unfold ons_mem in *. unfold unlift_ptt. des_ifs.
+  - ii. unfold ons_mem in *. unfold unlift_ptt. des_ifs.
+  - ii. unfold ons_mem in *. unfold unlift_ptt. des_ifs.
+  - ii. unfold ons_mem in *. unfold unlift_ptt. des_ifs.
 Qed.
 
 Global Program Instance SimMemInjOhLift: SimMemOhLift.class (@SimMemOh_default SimMemSV)
@@ -451,49 +628,44 @@ Lemma store_mapped
 .
 Proof.
   exploit Mem.store_mapped_inject; try apply MWF; eauto. i; des. inv MWF.
-  eexists (mk _ _ _ sm0.(ptt_src) sm0.(ptt_tgt)). dsplits; ss; eauto; cycle 1.
+  eexists (mk _ _ _ _ _ sm0.(ptt_src) sm0.(ptt_tgt)). dsplits; ss; eauto; cycle 1.
   - econs; ss; eauto.
+    + refl.
     + eapply Mem.store_unchanged_on; eauto. i.
-      specialize (PTTSRC blk_src i). apply proj1 in PTTSRC. hexploit1 PTTSRC; et.
+      specialize (PTTSRC blk_src i). hexploit1 PTTSRC; et.
       { unfold public_src, private_src. eapply or_not_and. left.
         unfold loc_unmapped. rewrite SIMBLK; ss. }
-      rr in PTTSRC. unfold external_src. rewrite PTTSRC. ss.
+      rr in PTTSRC. unfold ons_mem. rewrite PTTSRC. ss.
     + eapply Mem.store_unchanged_on; eauto. i.
-      specialize (PTTTGT blk_tgt i). apply proj1 in PTTTGT. hexploit1 PTTTGT; et.
+      specialize (PTTTGT blk_tgt i). hexploit1 PTTTGT; et.
       { unfold public_tgt, private_tgt. eapply or_not_and. left.
         unfold loc_out_of_reach. intro T. eapply T; et.
         apply Mem.store_valid_access_3 in STRSRC. destruct STRSRC. eauto with mem xomega.
       }
-      rr in PTTTGT. unfold external_tgt. rewrite PTTTGT. ss.
+      rr in PTTTGT. unfold ons_mem. rewrite PTTTGT. ss.
     + unfold public_src, private_src. ss. ii; des; eauto with mem.
-    + unfold public_tgt, private_tgt. ss. ii. eapply not_and_or in PR. des; eauto with mem.
-      unfold loc_out_of_reach in *. eapply PR; et. ii. eapply H1; et. eauto with mem.
-    + ii. eapply Mem.perm_store_2; eauto.
-    + ii. eapply Mem.perm_store_2; eauto.
+    + unfold public_tgt, private_tgt. ss. ii; des; eauto with mem.
   - des. econs; ss; eauto.
     + eapply Mem.store_unchanged_on; eauto. i.
-      specialize (PTTSRC blk_src i). apply proj1 in PTTSRC. hexploit1 PTTSRC; et.
+      specialize (PTTSRC blk_src i). hexploit1 PTTSRC; et.
       { unfold public_src, private_src. eapply or_not_and. left.
         unfold loc_unmapped. rewrite SIMBLK; ss. }
       rr in PTTSRC. unfold privmod_others. rewrite PTTSRC. ss.
     + eapply Mem.store_unchanged_on; eauto. i.
-      specialize (PTTTGT blk_tgt i). apply proj1 in PTTTGT. hexploit1 PTTTGT; et.
+      specialize (PTTTGT blk_tgt i). hexploit1 PTTTGT; et.
       { unfold public_tgt, private_tgt. eapply or_not_and. left.
         unfold loc_out_of_reach. intro T. eapply T; et.
         apply Mem.store_valid_access_3 in STRSRC. destruct STRSRC. eauto with mem xomega.
       }
       rr in PTTTGT. unfold privmod_others. rewrite PTTTGT. ss.
   - econs; ss; eauto.
-    + ii. etrans; try apply PTTSRC; et. unfold public_src, private_src. ss.
-      unfold valid_blocks. eapply iff_eta. do 2 apply f_equal. eapply prop_ext. eauto with mem.
-    + ii. etrans; try apply PTTTGT; et. unfold public_tgt, private_tgt. ss.
-      eapply iff_eta. do 1 apply f_equal. eapply prop_ext.
-      unfold valid_blocks, loc_out_of_reach.
-      split; ii; des.
-      * esplits; eauto with mem.
-        { ii. exploit H1; et. eauto with mem. }
-      * esplits; eauto with mem.
-        { ii. exploit H1; et. eauto with mem. }
+    + etrans; et. erewrite <- Mem.nextblock_store; et. xomega.
+    + etrans; et. erewrite <- Mem.nextblock_store; et. xomega.
+    + etrans; try apply PTTSRC; et. unfold public_src, private_src. ss.
+      unfold valid_blocks. ii. des. eauto with mem.
+    + etrans; try apply PTTTGT; et. unfold public_tgt, private_tgt. ss.
+      unfold valid_blocks. ii. des. eapply PR. esplits; eauto with mem.
+      { ii. exploit H1; et. eauto with mem. }
 Unshelve.
   all: try apply sm0.
 Qed.
@@ -544,49 +716,49 @@ Lemma free_parallel
 .
 Proof.
   exploit Mem.free_parallel_inject; try apply MWF; eauto. i; des. inv MWF.
-  assert(exists ptt_tgt: partition, True).
-  { esplits; et. exact (fun _ _ => pub). }
-  des.
-  eexists (mk _ _ _ sm0.(ptt_src) ptt_tgt0). dsplits; ss; eauto; cycle 1.
-  (* eexists (mk _ _ _ sm0.(ptt_src) sm0.(ptt_tgt)). dsplits; ss; eauto; cycle 1. *)
+  (* assert(exists ptt_tgt: partition, <<U: True>>). *)
+  (* { esplits; et. exact (fun _ _ => pub). } *)
+  (* des. *)
+  (* eexists (mk _ _ _ sm0.(ptt_src) ptt_tgt0). dsplits; ss; eauto; cycle 1. *)
+  eexists (mk _ _ _ _ _ sm0.(ptt_src) sm0.(ptt_tgt)). dsplits; ss; eauto; cycle 1.
   - econs; ss; eauto.
+    + refl.
     + eapply Mem.free_unchanged_on; eauto. i.
-      specialize (PTTSRC blk_src i). apply proj1 in PTTSRC. hexploit1 PTTSRC; et.
+      specialize (PTTSRC blk_src i). hexploit1 PTTSRC; et.
       { unfold public_src, private_src. eapply or_not_and. left.
         unfold loc_unmapped. rewrite SIMBLK; ss. }
-      rr in PTTSRC. unfold external_src. rewrite PTTSRC. ss.
+      rr in PTTSRC. unfold ons_mem. rewrite PTTSRC. ss.
     + eapply Mem.free_unchanged_on; eauto. i.
-      specialize (PTTTGT blk_tgt i). apply proj1 in PTTTGT. hexploit1 PTTTGT; et.
+      specialize (PTTTGT blk_tgt i). hexploit1 PTTTGT; et.
       { unfold public_tgt, private_tgt. eapply or_not_and. left.
         unfold loc_out_of_reach. intro T. eapply T; et.
         apply Mem.free_range_perm in FREESRC. eauto with mem xomega.
       }
-      rr in PTTTGT. unfold external_tgt. rewrite PTTTGT. ss.
-    + unfold public_src, private_src. ss. ii; des; eauto with mem.
-    + unfold public_tgt, private_tgt. ss. ii. eapply not_and_or in PR. des; eauto with mem.
-      unfold loc_out_of_reach in *. eapply PR; et. ii. eapply H2; et.
+      rr in PTTTGT. unfold ons_mem. rewrite PTTTGT. ss.
     + ii. eapply Mem.perm_free_3; eauto.
     + ii. eapply Mem.perm_free_3; eauto.
   - econs; ss; eauto.
-    + eapply Mem.unchanged_on_implies; try apply SPLITHINT3. i. rewrite PRIVSRC.
-      unfold privmod_others in *. des_ifs. eapply PTTSRC; et.
-      instantiate (1:= Some mi). ss. des_ifs. des_sumbool. ss.
-    + eapply Mem.unchanged_on_implies; try apply SPLITHINT3. i. rewrite PRIVTGT.
-      unfold privmod_others in *. des_ifs. eapply PTTTGT; et.
-      instantiate (1:= Some mi). ss. des_ifs. des_sumbool. ss.
+    + eapply Mem.free_unchanged_on; eauto. i.
+      specialize (PTTSRC blk_src i). hexploit1 PTTSRC; et.
+      { unfold public_src, private_src. eapply or_not_and. left.
+        unfold loc_unmapped. rewrite SIMBLK; ss. }
+      rr in PTTSRC. unfold privmod_others. rewrite PTTSRC. ss.
+    + eapply Mem.free_unchanged_on; eauto. i.
+      specialize (PTTTGT blk_tgt i). hexploit1 PTTTGT; et.
+      { unfold public_tgt, private_tgt. eapply or_not_and. left.
+        unfold loc_out_of_reach. intro T. eapply T; et.
+        apply Mem.free_range_perm in FREESRC. eauto with mem xomega.
+      }
+      rr in PTTTGT. unfold privmod_others. rewrite PTTTGT. ss.
   - econs; ss; eauto.
-    + etransitivity; eauto. unfold src_private. ss. ii; des. esplits; eauto.
-      unfold valid_blocks in *. eauto with mem.
-    + etransitivity; eauto. unfold tgt_private. ss. ii; des. esplits; eauto.
-      { ii. eapply PR. eauto with mem. eauto with mem. }
-      unfold valid_blocks in *. eauto with mem.
-    + etransitivity; eauto. erewrite <- Mem.nextblock_free; eauto. xomega.
-    + etransitivity; eauto. erewrite <- Mem.nextblock_free; eauto. xomega.
-    + etransitivity; eauto. unfold src_private. ss. ii; des. esplits; eauto.
-      unfold valid_blocks in *. eauto with mem.
-    + etransitivity; try apply PTTTGT; eauto. unfold tgt_private. ss. ii; des. esplits; eauto.
-      { ii. eapply PR. eauto with mem. eauto with mem. }
-      unfold valid_blocks in *. eauto with mem.
+    + etrans; et. erewrite <- Mem.nextblock_free; et. xomega.
+    + etrans; et. erewrite <- Mem.nextblock_free; et. xomega.
+    + etrans; try apply PTTSRC. unfold public_src, private_src; ss.
+      ii; des. eapply PR; esplits; et. unfold valid_blocks in *. eauto with mem.
+    + etrans; try apply PTTTGT. unfold public_tgt, private_tgt; ss.
+      ii; des. eapply PR; esplits; et.
+      { unfold loc_out_of_reach in *. ii. eapply H1; et. eauto with mem. }
+      { unfold valid_blocks in *. eauto with mem. }
 Unshelve.
   all: try apply sm0.
 Qed.
@@ -596,8 +768,6 @@ Lemma free_left
       (MWF: wf' sm0)
       (FREESRC: Mem.free sm0.(src) blk_src lo hi = Some m_src0)
       (SIMBLK: sm0.(inj) blk_src = Some (blk_tgt, delta))
-      (PRIVSRC: sm0.(src_external) = src_private sm0)
-      (PRIVTGT: sm0.(tgt_external) = tgt_private sm0)
   :
     exists sm1,
       (<<MSRC: sm1.(src) = m_src0>>)
@@ -609,81 +779,78 @@ Lemma free_left
 .
 Proof.
   exploit Mem.free_left_inject; try apply MWF; eauto. i; des. inv MWF.
-  eexists (mk _ _ _ _ _ _ _ _ _ _ _). dsplits; ss; eauto; cycle 1.
+  eexists (mk _ _ _ _ _ sm0.(ptt_src) sm0.(ptt_tgt)). dsplits; ss; eauto; cycle 1.
   - econs; ss; eauto.
-    + eapply Mem.free_unchanged_on; eauto.
-      ii. apply SRCEXT in H1. red in H1. des. red in H1. clarify.
-    + eapply Mem.unchanged_on_refl.
-    + eapply frozen_refl.
-    + eapply frozen_refl.
+    + refl.
+    + eapply Mem.free_unchanged_on; eauto. i.
+      specialize (PTTSRC blk_src i). hexploit1 PTTSRC; et.
+      { unfold public_src, private_src. eapply or_not_and. left.
+        unfold loc_unmapped. rewrite SIMBLK; ss. }
+      rr in PTTSRC. unfold ons_mem. rewrite PTTSRC. ss.
+    + refl.
     + ii. eapply Mem.perm_free_3; eauto.
   - econs; ss; eauto.
-    + eapply Mem.unchanged_on_implies; try apply SPLITHINT3. i. rewrite PRIVSRC.
-      unfold privmod_others in *. des_ifs. eapply PTTSRC; et.
-      instantiate (1:= Some mi). ss. des_ifs. des_sumbool. ss.
-    + eapply Mem.unchanged_on_implies; try apply SPLITHINT3. i. rewrite PRIVTGT.
-      unfold privmod_others in *. des_ifs. eapply PTTTGT; et.
-      instantiate (1:= Some mi). ss. des_ifs. des_sumbool. ss.
+    + eapply Mem.free_unchanged_on; eauto. i.
+      specialize (PTTSRC blk_src i). hexploit1 PTTSRC; et.
+      { unfold public_src, private_src. eapply or_not_and. left.
+        unfold loc_unmapped. rewrite SIMBLK; ss. }
+      rr in PTTSRC. unfold privmod_others. rewrite PTTSRC. ss.
+    + refl.
   - econs; ss; eauto.
-    + etransitivity; eauto. unfold src_private. ss. ii; des. esplits; eauto.
-      unfold valid_blocks in *. eauto with mem.
-    + etransitivity; eauto. unfold tgt_private. ss. ii; des. esplits; eauto.
-      { ii. eapply PR. eauto with mem. eauto with mem. }
-    + etransitivity; eauto. erewrite <- Mem.nextblock_free; eauto. xomega.
-    + etransitivity; eauto. unfold src_private. ss. ii; des. esplits; eauto.
-      unfold valid_blocks in *. eauto with mem.
-    + etransitivity; try apply PTTTGT; eauto. unfold tgt_private. ss. ii; des. esplits; eauto.
-      { ii. eapply PR. eauto with mem. eauto with mem. }
+    + etrans; et. erewrite <- Mem.nextblock_free; et. xomega.
+    + etrans; try apply PTTSRC. unfold public_src, private_src; ss.
+      ii; des. eapply PR; esplits; et. unfold valid_blocks in *. eauto with mem.
+    + etrans; try apply PTTTGT. unfold public_tgt, private_tgt; ss.
+      ii; des. eapply PR; esplits; et.
+      { unfold loc_out_of_reach in *. ii. eapply H0; et. eauto with mem. }
 Unshelve.
   all: try apply sm0.
 Qed.
 
-Lemma free_right
-      sm0 lo hi blk_tgt m_tgt0
-      (MWF: wf' sm0)
-      (FREETGT: Mem.free sm0.(tgt) blk_tgt lo hi = Some m_tgt0)
-      (PRIVTGT: forall ofs (BDD: lo <= ofs < hi), (tgt_private sm0) blk_tgt ofs)
-      (EXTTGT: forall ofs : Z, lo <= ofs < hi -> ~ tgt_external sm0 blk_tgt ofs)
-      (PRIVSRC: sm0.(src_external) = src_private sm0)
-      (PRIVTGT0: sm0.(tgt_external) = tgt_private sm0)
-  :
-    exists sm1,
-      (<<MSRC: sm1.(src) = sm0.(src)>>)
-      /\ (<<MTGT: sm1.(tgt) = m_tgt0>>)
-      /\ (<<MINJ: sm1.(inj) = sm0.(inj)>>)
-      /\ (<<MWF: wf' sm1>>)
-      /\ (<<MLE: le' sm0 sm1>>)
-      /\ (<<UNCH: SimMem.unch None sm0 sm1>>)
-.
-Proof.
-  exploit Mem.free_right_inject; try apply MWF; eauto.
-  { ii. eapply PRIVTGT in H1. red in H1. des. red in H1. eapply H1; eauto.
-    replace (ofs + delta - delta) with ofs by omega. eauto with mem.
-  }
-  i; des. inv MWF.
-  eexists (mk _ _ _ _ _ _ _ _ _ _ _). dsplits; ss; eauto; cycle 1.
-  - econs; ss; eauto.
-    + eapply Mem.unchanged_on_refl.
-    + eapply Mem.free_unchanged_on; eauto.
-    + eapply frozen_refl.
-    + eapply frozen_refl.
-    + ii. eapply Mem.perm_free_3; eauto.
-  - econs; ss; eauto.
-    + eapply Mem.unchanged_on_implies; try apply SPLITHINT3. i. rewrite PRIVSRC.
-      unfold privmod_others in *. des_ifs. eapply PTTSRC; et.
-      instantiate (1:= Some mi). ss. des_ifs. des_sumbool. ss.
-    + eapply Mem.unchanged_on_implies; try apply SPLITHINT3. i. rewrite PRIVTGT0.
-      unfold privmod_others in *. des_ifs. eapply PTTTGT; et.
-      instantiate (1:= Some mi). ss. des_ifs. des_sumbool. ss.
-  - econs; ss; eauto.
-    + etransitivity; eauto. unfold tgt_private. ss. ii; des. esplits; eauto.
-      unfold valid_blocks in *. eauto with mem.
-    + etransitivity; eauto. erewrite <- Mem.nextblock_free; eauto. xomega.
-    + etransitivity; try apply PTTTGT; eauto. unfold tgt_private. ss. ii; des. esplits; eauto.
-      unfold valid_blocks in *. eauto with mem.
-Unshelve.
-  all: try apply sm0.
-Qed.
+(* Lemma free_right *)
+(*       sm0 lo hi blk_tgt m_tgt0 *)
+(*       (MWF: wf' sm0) *)
+(*       (FREETGT: Mem.free sm0.(tgt) blk_tgt lo hi = Some m_tgt0) *)
+(*       (PRIVTGT: forall ofs (BDD: lo <= ofs < hi), (private_tgt sm0) blk_tgt ofs) *)
+(*       (EXTTGT: forall ofs : Z, lo <= ofs < hi -> ~ tgt_external sm0 blk_tgt ofs) *)
+(*   : *)
+(*     exists sm1, *)
+(*       (<<MSRC: sm1.(src) = sm0.(src)>>) *)
+(*       /\ (<<MTGT: sm1.(tgt) = m_tgt0>>) *)
+(*       /\ (<<MINJ: sm1.(inj) = sm0.(inj)>>) *)
+(*       /\ (<<MWF: wf' sm1>>) *)
+(*       /\ (<<MLE: le' sm0 sm1>>) *)
+(*       /\ (<<UNCH: SimMem.unch None sm0 sm1>>) *)
+(* . *)
+(* Proof. *)
+(*   exploit Mem.free_right_inject; try apply MWF; eauto. *)
+(*   { ii. eapply PRIVTGT in H1. red in H1. des. red in H1. eapply H1; eauto. *)
+(*     replace (ofs + delta - delta) with ofs by omega. eauto with mem. *)
+(*   } *)
+(*   i; des. inv MWF. *)
+(*   eexists (mk _ _ _ _ _ _ _ _ _ _ _). dsplits; ss; eauto; cycle 1. *)
+(*   - econs; ss; eauto. *)
+(*     + eapply Mem.unchanged_on_refl. *)
+(*     + eapply Mem.free_unchanged_on; eauto. *)
+(*     + eapply frozen_refl. *)
+(*     + eapply frozen_refl. *)
+(*     + ii. eapply Mem.perm_free_3; eauto. *)
+(*   - econs; ss; eauto. *)
+(*     + eapply Mem.unchanged_on_implies; try apply SPLITHINT3. i. rewrite PRIVSRC. *)
+(*       unfold privmod_others in *. des_ifs. eapply PTTSRC; et. *)
+(*       instantiate (1:= Some mi). ss. des_ifs. des_sumbool. ss. *)
+(*     + eapply Mem.unchanged_on_implies; try apply SPLITHINT3. i. rewrite PRIVTGT0. *)
+(*       unfold privmod_others in *. des_ifs. eapply PTTTGT; et. *)
+(*       instantiate (1:= Some mi). ss. des_ifs. des_sumbool. ss. *)
+(*   - econs; ss; eauto. *)
+(*     + etransitivity; eauto. unfold tgt_private. ss. ii; des. esplits; eauto. *)
+(*       unfold valid_blocks in *. eauto with mem. *)
+(*     + etransitivity; eauto. erewrite <- Mem.nextblock_free; eauto. xomega. *)
+(*     + etransitivity; try apply PTTTGT; eauto. unfold tgt_private. ss. ii; des. esplits; eauto. *)
+(*       unfold valid_blocks in *. eauto with mem. *)
+(* Unshelve. *)
+(*   all: try apply sm0. *)
+(* Qed. *)
 
 Lemma alloc_parallel
       sm0 lo_src hi_src lo_tgt hi_tgt blk_src m_src0
@@ -701,52 +868,127 @@ Lemma alloc_parallel
 .
 Proof.
   exploit Mem.alloc_parallel_inject; try apply MWF; eauto. i; des. inv MWF.
-  assert(FROZEN: frozen (inj sm0) f' (src_parent_nb sm0) (tgt_parent_nb sm0)).
-  {
-    + econs. ii. des. destruct (eq_block b_src blk_src).
-      * subst. rewrite H2 in NEW0. clarify. eapply Mem.alloc_result in ALCSRC. rewrite ALCSRC.
-        eapply Mem.alloc_result in H. rewrite H. esplits; eauto.
-      * rewrite H3 in NEW0; eauto. clarify.
-  }
-  eexists (mk _ _ f' _ _ _ _ _ _ _ _). exists b2.
+  (* assert(FROZEN: frozen (inj sm0) f' (src_parent_nb sm0) (tgt_parent_nb sm0)). *)
+  (* { *)
+  (*   + econs. ii. des. destruct (eq_block b_src blk_src). *)
+  (*     * subst. rewrite H2 in NEW0. clarify. eapply Mem.alloc_result in ALCSRC. rewrite ALCSRC. *)
+  (*       eapply Mem.alloc_result in H. rewrite H. esplits; eauto. *)
+  (*     * rewrite H3 in NEW0; eauto. clarify. *)
+  (* } *)
+  eexists (mk _ _ f' _ _
+              (fun b ofs => if eq_block b blk_src
+                                   then pub
+                                   else sm0.(ptt_src) b ofs)
+              (fun b ofs => if eq_block b b2
+                            then pub
+                            else sm0.(ptt_tgt) b ofs)). exists b2.
   dsplits; ss; eauto; cycle 1.
-  - econs; ss; eauto.
+  -
+    econs; ss; eauto.
+    + econs; eauto. econs; eauto. ii; des.
+      destruct (eq_block b_src blk_src).
+      * clarify. esplits; etrans; eauto with mem.
+        { exploit Mem.alloc_result; try apply ALCSRC. i; des. clarify. xomega. }
+        { exploit Mem.alloc_result; try apply H. i; des. clarify. xomega. }
+      * erewrite H3 in NEW0; et. clarify.
     + eapply Mem.alloc_unchanged_on; eauto.
     + eapply Mem.alloc_unchanged_on; eauto.
-    + eapply frozen_shortened; eauto.
+    + unfold ons_mem. ii. des_ifs.
+    + unfold ons_mem. ii. des_ifs.
+    + unfold ons_mem. ii. des_ifs.
+      exploit (PTTSRC blk_src x1).
+      { unfold public_src, private_src. apply or_not_and. right. ii. unfold valid_blocks in *.
+        eapply Mem.fresh_block_alloc; try eapply ALCSRC; eauto. }
+      unfold ons_mem. intro T. congruence.
+    + unfold ons_mem. ii. des_ifs.
+      exploit (PTTTGT b2 x1).
+      { unfold public_tgt, private_tgt. apply or_not_and. right. ii. unfold valid_blocks in *.
+        eapply Mem.fresh_block_alloc; try eapply H; eauto. }
+      unfold ons_mem. intro T. congruence.
+    + unfold ons_mem. ii. des_ifs.
+      exploit (PTTSRC blk_src x1).
+      { unfold public_src, private_src. apply or_not_and. right. ii. unfold valid_blocks in *.
+        eapply Mem.fresh_block_alloc; try eapply ALCSRC; eauto. }
+      unfold ons_mem. intro T. congruence.
+    + unfold ons_mem. ii. des_ifs.
+      exploit (PTTTGT b2 x1).
+      { unfold public_tgt, private_tgt. apply or_not_and. right. ii. unfold valid_blocks in *.
+        eapply Mem.fresh_block_alloc; try eapply H; eauto. }
+      unfold ons_mem. intro T. congruence.
     + ii. eapply Mem.perm_alloc_4; eauto.
       ii. subst b. eapply Mem.fresh_block_alloc; try eapply ALCSRC; eauto.
     + ii. eapply Mem.perm_alloc_4; eauto.
       ii. subst b. eapply Mem.fresh_block_alloc; eauto.
   - econs; ss; eauto.
-    + eapply Mem.unchanged_on_implies; try apply Mem_unchanged_on_bot; ss. eapply SPLITHINT3; et.
-    + eapply Mem.unchanged_on_implies; try apply Mem_unchanged_on_bot; ss. eapply SPLITHINT3; et.
+    + eapply Mem.alloc_unchanged_on; eauto.
+    + eapply Mem.alloc_unchanged_on; eauto.
+    + unfold privmods. ii. des_ifs. des_sumbool. clarify.
+      exploit (PTTSRC blk_src x1).
+      { unfold public_src, private_src. apply or_not_and. right. ii. unfold valid_blocks in *.
+        eapply Mem.fresh_block_alloc; try eapply ALCSRC; eauto. }
+      unfold ons_mem. intro T. congruence.
+    + unfold privmods. ii. des_ifs. des_sumbool. clarify.
+      exploit (PTTTGT b2 x1).
+      { unfold public_tgt, private_tgt. apply or_not_and. right. ii. unfold valid_blocks in *.
+        eapply Mem.fresh_block_alloc; try eapply ALCTGT; eauto. }
+      unfold ons_mem. intro T. congruence.
   - econs; ss; eauto.
-    + etransitivity; eauto. unfold src_private. ss. ii; des. esplits; eauto.
-      { destruct (eq_block x0 blk_src).
-        - subst x0. exfalso. eapply Mem.fresh_block_alloc; try eapply ALCSRC; eauto.
-        - r. rewrite H3; eauto. }
-      unfold valid_blocks in *. eauto with mem.
-    + etransitivity; eauto. unfold tgt_private. ss. ii; des. esplits; eauto.
-      { ii. destruct (eq_block b0 blk_src).
-        - subst b0. clarify. eapply Mem.fresh_block_alloc; eauto.
-        - eapply PR. rewrite <- H3; eauto. eauto with mem. }
-      unfold valid_blocks in *. eauto with mem.
-    + etransitivity; eauto. eapply Mem.nextblock_alloc in ALCSRC. rewrite ALCSRC. xomega.
-    + etransitivity; eauto. eapply Mem.nextblock_alloc in H. rewrite H. xomega.
-    + etransitivity; eauto. unfold src_private. ss. ii; des. esplits; eauto.
-      { destruct (eq_block x0 blk_src).
-        - subst x0. exfalso. eapply Mem.fresh_block_alloc; try eapply ALCSRC; eauto.
-        - r. rewrite H3; eauto. }
-      unfold valid_blocks in *. eauto with mem.
-    + etransitivity; try apply PTTTGT; eauto. unfold tgt_private. ss. ii; des. esplits; eauto.
-      { ii. destruct (eq_block b0 blk_src).
-        - subst b0. clarify. eapply Mem.fresh_block_alloc; eauto.
-        - eapply PR. rewrite <- H3; eauto. eauto with mem. }
-      unfold valid_blocks in *. eauto with mem.
+    + etrans; et. exploit Mem.nextblock_alloc; try apply ALCSRC. intro T; des. rewrite T. xomega.
+    + etrans; et. exploit Mem.nextblock_alloc; try apply H. intro T; des. rewrite T. xomega.
+    + unfold public_src, private_src in *. ss. ii. unfold ons_mem. des_ifs.
+      rewrite PTTSRC; ss. eapply not_and_or in PR. eapply or_not_and.
+      unfold valid_blocks in *.
+      des.
+      { left. ii. eapply PR. rr. rr in H4. erewrite H3; et. }
+      { right. ii. eapply PR. eauto with mem. }
+    + unfold public_tgt, private_tgt in *. ss. ii. unfold ons_mem. des_ifs.
+      rewrite PTTTGT; ss. eapply not_and_or in PR. eapply or_not_and.
+      unfold valid_blocks in *.
+      des.
+      { left. ii. eapply PR. rr. rr in H4. ii.
+        destruct (classic (b0 = blk_src)).
+        { clarify. }
+        erewrite H3 in H5; ss. eapply H4; et. eapply Mem.perm_alloc_4; et. }
+      { right. ii. eapply PR. eauto with mem. }
 Unshelve.
   all: try apply sm0.
 Qed.
+
+Require Import Classical_Pred_Type.
+
+Lemma not_and_or_strong
+      P Q
+      (H: (~ (P /\ Q)))
+  :
+    ((Q /\ ~ P) \/  ~Q)
+.
+Proof.
+  apply not_and_or in H.
+  destruct (classic Q); et.
+  des; clarify; et.
+Qed.
+
+Ltac Psimpl_ :=
+  match goal with
+  | [ H: ~ ~ ?P |- _ ] => apply NNPP in H
+  | [ H: (~?P -> ?P) |- _ ] => apply Peirce in H
+  | [ H: ~ (?P -> ?Q) |- _ ] => apply imply_to_and in H
+  | [ |- ~?P \/ ~?Q ] => apply imply_to_or
+  (* Parameter or_to_imply : forall P Q : Prop, ~ P \/ Q -> P -> Q. *)
+  | [ H: ~(?P /\ ?Q) |- _ ] => apply not_and_or_strong in H
+  | [ |- ~(?P /\ ?Q) ] => apply or_not_and
+  | [ H: ~(?P \/ ?Q) |- _ ] => apply not_or_and in H
+  | [ |- ~(?P \/ ?Q) ] => apply and_not_or
+  | [ H: ~(forall n, ~?P n) |- _ ] => apply not_all_not_ex in H
+  | [ H: ~(forall n, ?P n) |- _ ] => apply not_all_ex_not in H
+  | [ H: ~(exists n, ?P n) |- _ ] => apply not_ex_all_not in H
+  | [ H: ~(exists n, ~?P n) |- _ ] => apply not_ex_not_all in H
+  | [ |- ~(forall n, ?P n) ] => apply ex_not_not_all
+  | [ |- ~(exists n, ?P n) ] => apply all_not_not_ex
+  end
+.
+
+Ltac Psimpl := repeat Psimpl_.
 
 Lemma external_call
       sm0 ef se vargs t vres m_src0 tse vargs' vres' m_tgt0 f'
@@ -757,7 +999,12 @@ Lemma external_call
       (UNCHANGSRC: Mem.unchanged_on (loc_unmapped sm0.(inj)) sm0.(src) m_src0)
       (UNCHANGTGT: Mem.unchanged_on (loc_out_of_reach sm0.(inj) sm0.(src)) sm0.(tgt) m_tgt0)
       (INJINCR: inject_incr sm0.(inj) f')
-      (INJSEP: inject_separated sm0.(inj) f' sm0.(src) sm0.(tgt)):
+      (INJSEP: inject_separated sm0.(inj) f' sm0.(src) sm0.(tgt))
+      (PERMSRC: forall b ofs p, Mem.valid_block sm0.(src) b -> Mem.perm m_src0 b ofs Max p
+                                -> Mem.perm sm0.(src) b ofs Max p)
+      (PERMTGT: forall b ofs p, Mem.valid_block sm0.(tgt) b -> Mem.perm m_tgt0 b ofs Max p
+                                -> Mem.perm sm0.(tgt) b ofs Max p)
+  :
     exists sm1,
       (<<MSRC: sm1.(src) = m_src0>>)
       /\ (<<MTGT: sm1.(tgt) = m_tgt0>>)
@@ -768,81 +1015,106 @@ Lemma external_call
 .
 Proof.
   inv MWF.
-  assert (LE_LIFTED: le' (lift' sm0)
-                               (mk m_src0 m_tgt0 f' sm0.(ptt_src) sm0.(ptt_tgt)
-                                   (src_private sm0) (tgt_private sm0)
-                                   sm0.(src).(Mem.nextblock) sm0.(tgt).(Mem.nextblock)
-                                   sm0.(src_ge_nb) sm0.(tgt_ge_nb))).
-  { econs; ss; eauto.
-    - econs; i; eapply UNCHANGSRC; eauto; eapply H.
-    - econs; i; eapply UNCHANGTGT; eauto; eapply H.
-    - eapply frozen_shortened; try eapply inject_separated_frozen; eauto; try xomega.
-    - eapply inject_separated_frozen; eauto.
-    - ii. eapply external_call_max_perm; eauto.
-    - ii. eapply external_call_max_perm; eauto.
-  }
-  eexists (mk _ _ _ _ _ sm0.(src_external) sm0.(tgt_external) sm0.(src_parent_nb) sm0.(tgt_parent_nb) _ _); eauto.
-  dsplits; ss; eauto.
-  - econs; ss; eauto.
-    + etransitivity; eauto. eapply (after_private_src _ LE_LIFTED).
-    + etransitivity; eauto. eapply (after_private_tgt _ _ LE_LIFTED).
-    + eapply Ple_trans; eauto. eapply UNCHANGSRC.
-    + eapply Ple_trans; eauto; eapply UNCHANGTGT.
-    + etransitivity; eauto. eapply (after_private_src _ LE_LIFTED).
-    + etransitivity; try apply PTTTGT; eauto. eapply (after_private_tgt _ _ LE_LIFTED).
-  - exploit unlift_spec; eauto. econs; eauto.
-  - econs; ss; eauto.
-    + eapply Mem.unchanged_on_implies; try apply Mem_unchanged_on_bot; ss. eapply SPLITHINT3; et.
-    + eapply Mem.unchanged_on_implies; try apply Mem_unchanged_on_bot; ss. eapply SPLITHINT3; et.
+  eexists (mk _ _ _ sm0.(ge_nb_src) sm0.(ge_nb_tgt) sm0.(ptt_src) sm0.(ptt_tgt)); ss.
+  esplits; et.
+  - econs; et.
+    + ss. etrans; et. eapply Mem.unchanged_on_nextblock; et.
+    + ss. etrans; et. eapply Mem.unchanged_on_nextblock; et.
+    + unfold ons_mem. ss.
+      unfold public_src, private_src. ss.
+      ii. exploit PTTSRC; et. Psimpl. des.
+      * unfold public_src, private_src. Psimpl. ii. apply PR0. rr. rr in H.
+        destruct (f' x0) eqn:T; ss. destruct p; ss. exfalso.
+        exploit INJSEP; et. i; des. unfold valid_blocks in *. ss.
+      *
+        unfold public_src, private_src. Psimpl. ii. apply PR. unfold valid_blocks in *.
+        eapply Mem.valid_block_unchanged_on; et.
+    + unfold ons_mem. ss.
+      unfold public_tgt, private_tgt. ss.
+      ii. exploit PTTTGT; et. Psimpl. des.
+      * unfold public_tgt, private_tgt. Psimpl. ii. apply PR0. rr. rr in H. ii.
+        destruct (sm0.(inj) b0) eqn:T; ss.
+        { destruct p; ss. exploit INJINCR; et. i; clarify.
+          eapply H; et. eapply PERMSRC; et.
+          eapply NNPP. intro U. eapply Mem.mi_freeblocks in U; et. clarify. }
+        exploit INJSEP; et. i; des. unfold valid_blocks in *. ss.
+      *
+        unfold public_tgt, private_tgt. Psimpl. ii. apply PR. unfold valid_blocks in *.
+        eapply Mem.valid_block_unchanged_on; et.
+  - econs; ss; et.
+    + econs; et. eapply inject_separated_frozen in INJSEP. eapply frozen_shortened; et.
+    + eapply Mem.unchanged_on_implies; et.
+      ii. rr. destruct (sm0.(inj) b) eqn:T; ss. exfalso. destruct p; ss.
+      exploit PTTSRC; et.
+      { unfold public_src, private_src. unfold loc_unmapped. rewrite T. Psimpl. ii; clarify. }
+      i. unfold ons_mem in *. rewrite H in *. clarify.
+    + eapply Mem.unchanged_on_implies; et.
+      ii. rr. (* destruct (sm0.(inj) b) eqn:T; ss. exfalso. destruct p; ss. *)
+      exploit PTTTGT; et.
+      { unfold public_tgt, private_tgt. unfold loc_out_of_reach. Psimpl. ii; clarify.
+        eapply H3; et. }
+      i. unfold ons_mem in *. rewrite H in *. clarify.
+  - econs; ss; et.
+    + eapply Mem.unchanged_on_implies; et.
+      ii. rr. destruct (sm0.(inj) b) eqn:T; ss. exfalso. destruct p; ss.
+      exploit PTTSRC; et.
+      { unfold public_src, private_src. unfold loc_unmapped. rewrite T. Psimpl. ii; clarify. }
+      i. unfold ons_mem, privmod_others in *. rewrite H1 in *. clarify.
+    + eapply Mem.unchanged_on_implies; et.
+      ii. rr. (* destruct (sm0.(inj) b) eqn:T; ss. exfalso. destruct p; ss. *)
+      exploit PTTTGT; et.
+      { unfold public_tgt, private_tgt. unfold loc_out_of_reach. Psimpl. ii; clarify.
+        eapply H3; et. }
+      i. unfold ons_mem, privmod_others in *. rewrite H3 in *. clarify.
 Unshelve.
   all: by (try eapply inject_separated_frozen; eauto).
 Qed.
 
-Lemma free_list
-      sm0 l m_src0 l' m_tgt0
-      (MWF : wf' sm0)
-      (FREESRC: Mem.free_list sm0.(src) l = Some m_src0)
-      (FREETGT: Mem.free_list sm0.(tgt) l' = Some m_tgt0)
-      (MEMINJ: Mem.inject sm0.(inj) m_src0 m_tgt0)
-      (EXTSRC: forall b lo hi i, In (b, lo, hi) l -> lo <= i < hi -> ~ sm0.(src_external) b i)
-      (EXTTGT: forall b lo hi i, In (b, lo, hi) l' -> lo <= i < hi -> ~ sm0.(tgt_external) b i):
-    exists sm1,
-      (<<MSRC: sm1.(src) = m_src0>>)
-      /\ (<<MTGT: sm1.(tgt) = m_tgt0>>)
-      /\ (<<MINJ: sm1.(inj) = sm0.(inj)>>)
-      /\ (<<MWF: wf' sm1>>)
-      /\ (<<MLE: le' sm0 sm1>>)
-      /\ (<<UNCH: SimMem.unch None sm0 sm1>>)
-.
-Proof.
-  inv MWF. eexists (mk _ _ _ _ _ _ _ _ _ _ _). dsplits; ss; eauto; cycle 1.
-  - econs; ss; eauto.
-    + eapply Mem.free_list_unchanged_on; eauto.
-    + eapply Mem.free_list_unchanged_on; eauto.
-    + eapply frozen_refl. + eapply frozen_refl.
-    + ii. eapply Mem.perm_free_list; eauto.
-    + ii. eapply Mem.perm_free_list; eauto.      
-  - econs; ss; eauto.
-    + eapply Mem.unchanged_on_implies; try apply Mem_unchanged_on_bot; ss. eapply SPLITHINT3; et.
-    + eapply Mem.unchanged_on_implies; try apply Mem_unchanged_on_bot; ss. eapply SPLITHINT3; et.
-  - econs; ss; eauto.
-    + etransitivity; eauto. unfold src_private. ii. ss. des. esplits; eauto.
-      red. red. erewrite Mem.free_list_nextblock; eauto.
-    + etransitivity; eauto. unfold tgt_private. ii. ss. des. esplits; eauto.
-      red. ii. eapply PR; eauto.
-      exploit Mem.perm_free_list; try eapply FREESRC; eauto. i; des. ss.
-      red. red. erewrite Mem.free_list_nextblock; eauto.
-    + erewrite Mem.free_list_nextblock; eauto.
-    + erewrite Mem.free_list_nextblock; eauto.
-    + etransitivity; eauto. unfold src_private. ii. ss. des. esplits; eauto.
-      red. red. erewrite Mem.free_list_nextblock; eauto.
-    + etransitivity; try apply PTTTGT; eauto. unfold tgt_private. ii. ss. des. esplits; eauto.
-      red. ii. eapply PR; eauto.
-      exploit Mem.perm_free_list; try eapply FREESRC; eauto. i; des. ss.
-      red. red. erewrite Mem.free_list_nextblock; eauto.
-Unshelve.
-  all: try apply sm0.
-Qed.
+(* Lemma free_list *)
+(*       sm0 l m_src0 l' m_tgt0 *)
+(*       (MWF : wf' sm0) *)
+(*       (FREESRC: Mem.free_list sm0.(src) l = Some m_src0) *)
+(*       (FREETGT: Mem.free_list sm0.(tgt) l' = Some m_tgt0) *)
+(*       (MEMINJ: Mem.inject sm0.(inj) m_src0 m_tgt0) *)
+(*       (EXTSRC: forall b lo hi i, In (b, lo, hi) l -> lo <= i < hi -> ~ sm0.(src_external) b i) *)
+(*       (EXTTGT: forall b lo hi i, In (b, lo, hi) l' -> lo <= i < hi -> ~ sm0.(tgt_external) b i): *)
+(*     exists sm1, *)
+(*       (<<MSRC: sm1.(src) = m_src0>>) *)
+(*       /\ (<<MTGT: sm1.(tgt) = m_tgt0>>) *)
+(*       /\ (<<MINJ: sm1.(inj) = sm0.(inj)>>) *)
+(*       /\ (<<MWF: wf' sm1>>) *)
+(*       /\ (<<MLE: le' sm0 sm1>>) *)
+(*       /\ (<<UNCH: SimMem.unch None sm0 sm1>>) *)
+(* . *)
+(* Proof. *)
+(*   inv MWF. eexists (mk _ _ _ _ _ _ _ _ _ _ _). dsplits; ss; eauto; cycle 1. *)
+(*   - econs; ss; eauto. *)
+(*     + eapply Mem.free_list_unchanged_on; eauto. *)
+(*     + eapply Mem.free_list_unchanged_on; eauto. *)
+(*     + eapply frozen_refl. + eapply frozen_refl. *)
+(*     + ii. eapply Mem.perm_free_list; eauto. *)
+(*     + ii. eapply Mem.perm_free_list; eauto.       *)
+(*   - econs; ss; eauto. *)
+(*     + eapply Mem.unchanged_on_implies; try apply Mem_unchanged_on_bot; ss. eapply SPLITHINT3; et. *)
+(*     + eapply Mem.unchanged_on_implies; try apply Mem_unchanged_on_bot; ss. eapply SPLITHINT3; et. *)
+(*   - econs; ss; eauto. *)
+(*     + etransitivity; eauto. unfold src_private. ii. ss. des. esplits; eauto. *)
+(*       red. red. erewrite Mem.free_list_nextblock; eauto. *)
+(*     + etransitivity; eauto. unfold tgt_private. ii. ss. des. esplits; eauto. *)
+(*       red. ii. eapply PR; eauto. *)
+(*       exploit Mem.perm_free_list; try eapply FREESRC; eauto. i; des. ss. *)
+(*       red. red. erewrite Mem.free_list_nextblock; eauto. *)
+(*     + erewrite Mem.free_list_nextblock; eauto. *)
+(*     + erewrite Mem.free_list_nextblock; eauto. *)
+(*     + etransitivity; eauto. unfold src_private. ii. ss. des. esplits; eauto. *)
+(*       red. red. erewrite Mem.free_list_nextblock; eauto. *)
+(*     + etransitivity; try apply PTTTGT; eauto. unfold tgt_private. ii. ss. des. esplits; eauto. *)
+(*       red. ii. eapply PR; eauto. *)
+(*       exploit Mem.perm_free_list; try eapply FREESRC; eauto. i; des. ss. *)
+(*       red. red. erewrite Mem.free_list_nextblock; eauto. *)
+(* Unshelve. *)
+(*   all: try apply sm0. *)
+(* Qed. *)
 
 End ORIGINALS.
 
@@ -854,16 +1126,14 @@ Record mcompat (sm0: t') (m_src0 m_tgt0: mem) (F: meminj): Prop := mkmcompat {
 
 End MEMINJ.
 
+Hint Unfold ons_mem.
 Hint Unfold valid_blocks.
-Hint Unfold src_private tgt_private.
+Hint Unfold lift_ptt unlift_ptt lift' unlift'.
+Hint Unfold private_src private_tgt.
+Hint Unfold public_src public_tgt.
 
 Ltac compat_tac := ss; econs; eauto; try congruence.
 
-Ltac spl := esplits; [|reflexivity].
-Ltac spl_approx sm :=
-  eexists (mk _ _ _ sm.(src_external) sm.(tgt_external) sm.(src_parent_nb) sm.(tgt_parent_nb) sm.(src_ge_nb) sm.(tgt_ge_nb)); splits; eauto.
-Ltac spl_exact sm :=
-  exists sm; splits; [|try etransitivity; eauto; try reflexivity; eauto].
 
 
 
@@ -891,8 +1161,11 @@ Inductive sim_skenv_inj (sm: SimMem.t) (__noname__: SimSymbId.t') (skenv_src ske
     (* (BOUNDSRC: Ple skenv_src.(Genv.genv_next) sm.(src_parent_nb)) *)
     (* (BOUNDTGT: Ple skenv_src.(Genv.genv_next) sm.(tgt_parent_nb)) *)
     (SIMSKENV: SimSymbId.sim_skenv skenv_src skenv_tgt)
-    (NBSRC: skenv_src.(Genv.genv_next) = sm.(src_ge_nb))
-    (NBTGT: skenv_tgt.(Genv.genv_next) = sm.(tgt_ge_nb)).
+    (PTTSRC: forall b ofs (LE: Plt b skenv_src.(Genv.genv_next)), sm.(ptt_src) b ofs = pub)
+    (PTTTGT: forall b ofs (LE: Plt b skenv_tgt.(Genv.genv_next)), sm.(ptt_tgt) b ofs = pub)
+    (NBSRC: skenv_src.(Genv.genv_next) = sm.(ge_nb_src))
+    (NBTGT: skenv_tgt.(Genv.genv_next) = sm.(ge_nb_tgt))
+.
 
 Section REVIVE.
 
@@ -911,6 +1184,7 @@ End REVIVE.
 
 
 
+
 Global Program Instance SimSymbId: SimSymb.class SimMemSV := {
   t := SimSymbId.t';
   src := SimSymbId.src;
@@ -924,8 +1198,11 @@ Next Obligation. eapply SimSymbId.wf_link; eauto. Qed.
 Next Obligation. inv SIMSKE. inv SIMSKENV. ss. Qed.
 Next Obligation.
   exploit SimSymbId.wf_load_sim_skenv; eauto. i; des.
-  eexists. eexists (mk m_src m_src (Mem.flat_inj m_src.(Mem.nextblock)) (fun _ _ => etc) (fun _ _ => etc)
-                       bot2 bot2 m_src.(Mem.nextblock) m_src.(Mem.nextblock) m_src.(Mem.nextblock) m_src.(Mem.nextblock)). ss.
+  eexists.
+  eexists (mk m_src m_src (Mem.flat_inj m_src.(Mem.nextblock))
+              m_src.(Mem.nextblock)
+              m_src.(Mem.nextblock)
+              (fun _ _ => pub) (fun _ _ => pub)); ss.
   esplits; ss; eauto.
   - econs; ss; eauto.
     + econs; eauto; ii; ss.
@@ -935,8 +1212,8 @@ Next Obligation.
     + ss. erewrite ! Genv.init_mem_genv_next; eauto.
   - econs; ss; try xomega; ii; des; ss; eauto.
     + eapply Genv.initmem_inject; eauto; (u in *; eauto).
-    + unfold privmods in *. des_ifs.
-    + unfold privmods in *. des_ifs.
+    (* + unfold privmods in *. des_ifs. *)
+    (* + unfold privmods in *. des_ifs. *)
   - rewrite MAINSIM. unfold Genv.symbol_address. des_ifs. unfold Mem.flat_inj. econs; eauto.
     + des_ifs. exfalso. apply n. eapply Plt_Ple_trans.
       { eapply Genv.genv_symb_range; et. }
@@ -946,8 +1223,10 @@ Qed.
 Next Obligation.
   inv SIMSKENV. inv INJECT. econs; eauto. econs; eauto.
   - ii. exploit DOMAIN; eauto. i. eapply MLE; eauto.
-  - ii. inv MLE. eapply IMAGE; eauto. erewrite frozen_preserves_tgt; eauto.
+  - ii. inv MLE. inv FINCR. eapply IMAGE; eauto. erewrite frozen_preserves_tgt; eauto.
     eapply Plt_Ple_trans; eauto. rewrite <- NBTGT. rr in SIMSKENV0. clarify. refl.
+  - inv MLE. ii. eapply PUBSRC. r. et.
+  - inv MLE. ii. eapply PUBTGT. r. et.
   - inv MLE. eauto with congruence.
   - inv MLE. eauto with congruence.
 Qed.
@@ -988,40 +1267,54 @@ Next Obligation.
   i; des. do 2 eexists. dsplits; eauto; ss.
   - instantiate (1:= Retv.mk _ _); ss. eapply external_call_symbols_preserved; eauto.
     eapply SimSymbId.sim_skenv_equiv; eauto. eapply SIMSKENV.
-  - destruct retv_src; ss. instantiate (1:= mk _ _ _ _ _ _ _ _ _ _ _). econs 1; ss; eauto.
+  - destruct retv_src; ss. instantiate (1:= mk _ _ _ _ _ ptt_src0 ptt_tgt0). econs 1; ss; eauto.
     instantiate (1:= (Retv.m retv_src)). ss.
-  - assert(FROZEN: frozen inj0 f' src_parent_nb0 tgt_parent_nb0).
-    { eapply inject_separated_frozen in H5. inv H5. econs; eauto. i.
-      exploit NEW_IMPLIES_OUTSIDE; eauto. i; des. esplits; xomega. }
+  - assert(FROZEN: frozen inj0 f' ge_nb_src0 ge_nb_tgt0).
+    { eapply inject_separated_frozen in H5. eapply frozen_shortened; eauto. }
     econs; ss; eauto.
-    + eapply Mem.unchanged_on_implies; eauto. u. i; des; ss. eapply SRCEXT in H6. unfold src_private in *. ss. des; ss.
-    + eapply Mem.unchanged_on_implies; eauto. u. i; des; ss. eapply TGTEXT in H6. unfold tgt_private in *. ss. des; ss.
-    + eapply frozen_shortened; et.
+    + eapply Mem.unchanged_on_implies; eauto. u. i; des; ss. r.
+      destruct (inj0 b) eqn:T; ss. destruct p; ss. exfalso.
+      exploit PTTSRC; et.
+      { unfold public_src, private_src; ss. intro U. des. r in U. rewrite T in U; ss. }
+      intro U. r in U. rewrite U in *. ss.
+    + eapply Mem.unchanged_on_implies; eauto. u. i; des; ss. r.
+      ii as T.
+      exploit PTTTGT; et.
+      { unfold public_tgt, private_tgt; ss. intro U. des. r in U. exploit U; et. }
+      intro U. r in U. rewrite U in *. ss.
     + ii. eapply external_call_max_perm; eauto.
     + ii. eapply external_call_max_perm; eauto.
-  (* - econs; ii; ss. *)
-  (*   + eapply Mem.unchanged_on_implies. *)
-  (*     { eapply Mem_unchanged_on_bot; et. eapply SPLITHINT1. } *)
-  (*     ss. *)
-  (*   + eapply Mem.unchanged_on_implies. *)
-  (*     { eapply Mem_unchanged_on_bot; et. eapply SPLITHINT1. } *)
-  (*     ss. *)
-  - econs; ss; eauto.
+  - econs; ii; ss.
+    + eapply Mem.unchanged_on_implies; eauto. u. i; des; ss. r.
+      destruct (inj0 b) eqn:T; ss. destruct p; ss. exfalso.
+      exploit PTTSRC; et.
+      { unfold public_src, private_src; ss. intro U. des. r in U. rewrite T in U; ss. }
+      intro U. r in U. rewrite U in *. ss.
+    + eapply Mem.unchanged_on_implies; eauto. u. i; des; ss. r.
+      ii as T.
+      exploit PTTTGT; et.
+      { unfold public_tgt, private_tgt; ss. intro U. des. r in U. exploit U; et. }
+      intro U. r in U. rewrite U in *. ss.
   - apply inject_separated_frozen in H5. econs; ss.
-    (* + eapply after_private_src; ss; eauto. *)
-    (* + eapply after_private_tgt; ss; eauto. *)
-    + etrans; eauto. unfold src_private. ss. ii. des. esplits; eauto.
-      * rr. rr in PR. destruct (f' x0) eqn:T; ss. destruct p; ss. inv H5.
-        exploit NEW_IMPLIES_OUTSIDE; eauto. i. des. unfold valid_blocks in *. unfold Mem.valid_block in *. xomega.
-      * r. eapply Mem.valid_block_unchanged_on; et.
-    + etrans; eauto. unfold tgt_private. ss. ii. des. esplits; eauto.
-      * rr. rr in PR. ii. destruct (inj0 b0) eqn:T; ss.
-        -- destruct p; ss. exploit H4; eauto. i; clarify.
-           eapply PR; et. eapply external_call_max_perm; et. eapply Mem.valid_block_inject_1; try apply T; et.
-        -- inv H5. exploit NEW_IMPLIES_OUTSIDE; eauto. i. des. unfold valid_blocks in *. unfold Mem.valid_block in *. xomega.
-      * r. eapply Mem.valid_block_unchanged_on; et.
     + inv H2. xomega.
     + inv H3. xomega.
+    + unfold public_src, private_src; ss. sii T.
+      exploit PTTSRC; et.
+      unfold public_src, private_src; ss. sii T; des.
+      eapply PR. esplits; et.
+      * eapply loc_unmapped_frozen; et.
+      * unfold valid_blocks in *.
+        eapply Plt_Ple_trans; et.
+        eapply Mem.unchanged_on_nextblock; et.
+    + unfold public_tgt, private_tgt; ss. sii T.
+      exploit PTTTGT; et.
+      unfold public_tgt, private_tgt; ss. sii T; des.
+      eapply PR. esplits; et.
+      * eapply loc_out_of_reach_frozen; et.
+        sii U. eapply external_call_max_perm; et. eapply Mem.valid_block_inject_1; et.
+      * unfold valid_blocks in *.
+        eapply Plt_Ple_trans; et.
+        eapply Mem.unchanged_on_nextblock; et.
 Unshelve.
   all: ss.
 Qed.
